testsuite/tests/coqgen/sortproof.v
@@ -3,18 +3,21 @@ Require Import Sint63 Ascii String Floats cocti_defs test2.
 
 Axiom funext : forall A B (f g : A -> B), f =1 g -> f = g.
 
+Lemma happly [A B] [f g : A -> B] x : f = g -> f x = g x.
+Proof. by move=> ->. Qed.
+
 Lemma bindretf A B (a : A) (f : A -> M B) : Ret a >>= f = f a.
-Proof.
-  rewrite /Bind /=.
-  exact: funext.
-Qed.
+Proof. exact: funext. Qed.
 
 Lemma bindmret A (m : M A) : m >>= Ret = m.
 Proof.
-  rewrite /Bind /=.
+  rewrite /Bind.
   apply funext => env /=.
   by case: (m env) => env' [] r.
 Qed.
+
+Lemma bindfailf A B e (g : A -> M B) : @Fail A e >>= g = @Fail B e.
+Proof. exact: funext. Qed.
 
 Definition fmap A B (f : A -> B) (m : M A) : M B :=
   m >>= fun a => Ret (f a).
@@ -44,7 +47,25 @@ Fixpoint sorted l := (* all を使って bool 上の述語を定義する *)
 Lemma compare_ok h x y : ml_le h.+1 ml_int x y = Ret (le x y).
 Proof. exact: funext. Qed.
 
-Lemma insert_pure h b l l' env env' : insert h ml_int b l env = Ret l' env'
+Definition pure [T] (m : M T) :=
+  (exists r, m = Ret r) \/ (exists e, m = Fail e).
+
+Lemma insert_pure h b l : pure (insert h ml_int b l).
+Proof.
+  elim: h l => [| h IH] l.
+  - by right; eexists.
+  - case: l.
+    + by left; eexists.
+    + move=> a l /=.
+      destruct h.
+      - by right; eexists.
+      - rewrite compare_ok bindretf.
+        case: ifPn => _.
+        + by left; eexists.
+        + case: (IH l) => -[c ->]; [left|right]; by eexists.
+Qed.
+
+(*Lemma insert_pure h b l l' env env' : insert h ml_int b l env = Ret l' env'
   -> insert h ml_int b l = Ret l'.
 Proof.
   elim: h l l' => //= h IH [l [] _ <-|a l l'] //.
@@ -58,9 +79,6 @@ Proof.
   by rewrite (IH l a0) // H henv.
 Qed.
 
-Lemma happly [A B] [f g : A -> B] x : f = g -> f x = g x.
-Proof. by move=> ->. Qed.
-
 Corollary insert_env h b l l' env env' :
  insert h ml_int b l env = Ret l' env' -> env = env'.
 Proof.
@@ -68,9 +86,23 @@ Proof.
   move:(H) => /insert_pure.
   move/(happly env).
   by rewrite H => -[] <-.
+Qed.*)
+
+Lemma isort_pure h l : pure (isort h ml_int l).
+Proof.
+  elim: h l => [| h IH [|a l]] /=.
+  - by right; eexists.
+  - by left; eexists.
+  - destruct h.
+    + by right; eexists.
+    + case: (IH l) => -[b ->].
+      - rewrite bindretf.
+        exact: insert_pure.
+      - right.
+        by exists b; rewrite bindfailf.
 Qed.
 
-Lemma isort_pure h l l' env env' : isort h ml_int l env = Ret l' env'
+(*Lemma isort_pure h l l' env env' : isort h ml_int l env = Ret l' env'
   -> isort h ml_int l = Ret l'.
 Proof.
   elim: h l l' => // h IH [_ [] _ <- |a l l'] //=.
@@ -83,25 +115,23 @@ Proof.
   + rewrite H.
     move:H'.
     by move /insert_env <-.
-Qed.
+Qed.*)
 
 Lemma le_seq_insert h a b l l' : insert h ml_int b l = Ret l' ->
   le a b -> all (le a) l -> all (le a) l'.
-Proof.
+Proof. (*not_use_empty_env*)
   elim: h l l' => /= [_ _ |h IH [|c l] l'] /(happly empty_env) //.
   - by move=> -[] /= <- /= ->.
-  - rewrite /Bind.
-    destruct h => //.
-    rewrite compare_ok (lock (h.+1)) /=.
+  - destruct h => //.
+    rewrite compare_ok bindretf.
     case: ifPn.
     + move=> lebc [] <- leab /andP [] leac leall /=.
       by rewrite leab leac.
     + move=> nlebc.
-      rewrite -lock.
-      move H : (insert h.+1 ml_int b l empty_env) => [env' r].
-      case: r H => // l'' H [] henv <- leab /andP [] leac leall /=.
-      move/ insert_pure /IH in H.
-      by rewrite leac H.
+      case: (insert_pure h.+1 b l) => -[d H].
+      - rewrite H bindretf => -[] <- /= leab /andP [] leac leall /=.
+        by rewrite leac (IH l d).
+      - by rewrite H bindfailf.
 Qed.
 
 Lemma eq_intP : Equality.axiom (fun (x y : int) => (x =? y)%sint63).
@@ -151,36 +181,105 @@ Qed.
 Lemma insert_ok h a l l' : insert h ml_int a l = Ret l' ->
   sorted l -> sorted l'.
 Proof.
-  elim: h l l' => [_ _ |h IH[|c l] l'] /(happly empty_env) //=.
+  elim: h l l' => [_ _ |h IH[|b l] l'] /(happly empty_env) //=.
   - by move=> [] <-.
   - destruct h => //.
-    rewrite compare_ok (lock (h.+1)) /=.
-    rewrite bindretf.
+    rewrite compare_ok bindretf.
     case: ifPn.
-    + move=> leac [] <- /andP [] leall sortedl /=.
-      by rewrite leac leall sortedl (le_seq_trans a c l).
+    + move=> leab [] <- /andP [] leall sortedl /=.
+      by rewrite leab leall sortedl (le_seq_trans a b l).
     + move=> nleac.
-      rewrite -lock /Bind.
-      move H : (insert h.+1 ml_int a l empty_env) => [env' r].
-      case: r H => // l'' H [] henv <- /andP [] leall sortedl /=.
-      apply /andP.
-      split.
-      - rewrite (le_seq_insert h.+1 c a l l'') //.
-        by apply (insert_pure _ _ _ _ empty_env env').
+      case: (insert_pure h.+1 a l) => -[l'' H].
+      - rewrite H bindretf => -[] <- /andP [] leall sortedl /=.
+        rewrite (le_seq_insert h.+1 b a l l'') //.
+        rewrite (IH l l'') //.
         by apply le_total.
-      - move/ insert_pure /IH in H.
-        by rewrite H.
+      - by rewrite H bindfailf.
 Qed.
 
 Theorem isort_ok h l l' : isort h ml_int l = Ret l' -> sorted l'.
 Proof.
-  elim: h l l' => [_ _ |h IH [|c l] l'] /(happly empty_env) //=.
+  elim: h l l' => [_ _ |h IH [|a l] l'] /(happly empty_env) //=.
   - by move=> [] <-.
-  - rewrite /Bind.
-    destruct h => //.
-    move H : (isort h.+1 ml_int l empty_env) => [env r].
-    case: r H => // l'' H H'.
-    apply (insert_ok h.+1 c l'' l').
-    - apply /(insert_pure _ _ _ _ env empty_env) /H'.
-    - apply /(IH l l'') /(isort_pure _ _ _ empty_env env) /H.
+  - destruct h => //.
+    case: (isort_pure h.+1 l) => -[l'' H].
+    + rewrite H bindretf.
+      case: (insert_pure h.+1 a l'') => -[l0 H'].
+      - rewrite H' => -[] <-.
+        by apply /(insert_ok h.+1 a l'' l0) /(IH l l'').
+      - by rewrite H'.
+    + by rewrite H bindfailf.
+Qed.
+End Sort.
+
+Section perm.
+Inductive Permutation {T} : seq T -> seq T -> Prop :=
+  | perm_nil : Permutation nil nil
+  | perm_skip : forall x l l',
+  Permutation l l' -> Permutation (x::l) (x::l')
+  | perm_swap : forall x y l, Permutation (x::y::l) (y::x::l)
+  | perm_trans : forall l l' l'',
+  Permutation l l'
+  -> Permutation l' l'' -> Permutation l l''.
+
+Lemma perm_refl A (l : seq A) : Permutation l l.
+Proof.
+  elim l.
+  - by apply perm_nil.
+  - move=> a l' H.
+    by apply perm_skip.
+Qed.
+
+Hint Constructors Permutation.
+
+Lemma ret_inj [T] (x y : T) : Ret x = Ret y -> x = y.
+Proof. by move /(happly empty_env) => []. Qed.
+
+Lemma failret [T] (a : T) (e : Env.Exn) : Fail e = Ret a -> false.
+Proof. by move/(happly empty_env). Qed.
+
+Theorem insert_perm h l a l' :
+  insert h ml_int a l = Ret l' -> Permutation (a :: l) l'.
+Proof.
+  elim : h l l' => [l l' | h IH [|b l] l'] //=. (*move/ret_inj_ver*)
+  - by move/(failret _).
+  - move/(ret_inj _ _) <-; auto.
+  - destruct h => //.
+    + rewrite /ml_le /wrap_compare bindfailf.
+      by move/(failret _).
+    + rewrite compare_ok bindretf.
+      case: ifPn => _.
+      - move/(ret_inj _ _) <-.
+        exact: perm_refl.
+      - case: (insert_pure h.+1 a l) => -[c H].
+        + rewrite H bindretf.
+          move/(ret_inj _ _) <-; eauto.
+        + rewrite H bindfailf.
+          by move/(failret _).
+Restart.
+  elim: h l l' => [_ _ | h IH [|b l] l'] /(happly empty_env) //=.
+  - move=> [] <-; auto.
+  - destruct h => //.
+    rewrite compare_ok bindretf.
+    case: ifPn => H.
+    + move=> [] <-.
+      apply perm_refl.
+    + case: (insert_pure h.+1 a l) => -[c H'].
+      - rewrite H' bindretf.
+        move => [] <-; eauto.
+      - by rewrite H' bindfailf.
+Qed.
+
+Theorem isort_perm h l l' :
+  isort h ml_int l = Ret l' -> Permutation l l'.
+Proof.
+  elim: h l l' => [l l' | h IH [|a l] l'] //=.
+  - by move/(failret l').
+  - move/(ret_inj _ _) <-; auto.
+  - destruct h.
+    + rewrite /isort bindfailf.
+      by move/(failret _).
+    + case: (isort_pure h.+1 l) => -[l'' H].
+      - rewrite H bindretf.
+        
 Qed.
