testsuite/tests/coqgen/test2.v
@@ -19,7 +19,6 @@ Inductive ml_type :=
   | ml_t0
   | ml_t1
   | ml_t2
-  | ml_prod (_ : ml_type) (_ : ml_type)
   | ml_lazy_val (_ : ml_type)
   | ml_ref (_ : ml_type)
   | ml_arrow (_ : ml_type) (_ : ml_type).
@@ -56,8 +55,6 @@ Inductive t2 := T0 (_ : t0)
 with t0 := | O | T1_1 (_ : t1)
 with t1 := T2_1 (_ : t2).
 
-Inductive prod (a : Type) (b : Type) := Pair (_ : a) (_ : b).
-
 
 Inductive lazy_val (a : Type) :=
   LzVal of a | LzThunk of M a | LzExn of ml_exns.
@@ -82,7 +79,6 @@ Fixpoint coq_type (T : ml_type) : Type :=
   | ml_t0 => t0
   | ml_t1 => t1
   | ml_t2 => t2
-  | ml_prod T1 T2 => prod (coq_type T1) (coq_type T2)
   | ml_lazy_val T1 => lazy_val (coq_type T1)
   | ml_ref T1 => loc T1
   | ml_arrow T1 T2 => coq_type T1 -> M (coq_type T2)
@@ -153,12 +149,6 @@ Fixpoint compare_rec (h : nat) (T : ml_type)
     | ml_t2 =>
       fun x y =>
         match x, y with | T0 x1, T0 y1 => compare_rec ml_t0 x1 y1 end
-    | ml_prod T1 T2 =>
-      fun x y =>
-        match x, y with
-        | Pair x1 x2, Pair y1 y2 =>
-          lexi_compare (compare_rec T1 x1 y1) (Delay (compare_rec T2 x2 y2))
-        end
     | ml_lazy_val T1 =>
       fun x y => Fail (Catchable (Invalid_argument "compare"%string))
     | ml_ref T1 => fun x y => compare_ref compare_rec T1 x y
@@ -269,3 +259,9 @@ Fixpoint isort (h : nat) (T_1 : ml_type) (l_1 : coq_type (ml_list T_1))
     | a :: l' => do v <- isort h T_1 l'; insert h T_1 a v
     end
   else FailGas.
+
+Fixpoint gcd (h : nat) (m n : coq_type ml_int) : M (coq_type ml_int) :=
+  if h is h.+1 then
+    do v <- ml_eq h ml_int m 0%int63; if v then Ret n else gcd h (mods n m) m
+  else FailGas.
+
